Move SSA correctness-related material to a separate source file
Also remove the dependence in the moved material on the VariablesSSA
class and start changing the signatures such that there will be no need
to repeatedly split the live-on-entry and live-on-exit instances into
separate subsets (XL1i-XL4i and XL4f-XL5f).

SSA.dfy
@@ -1,7 +1,7 @@
 include "Definitions.dfy"
 include "Substitutions.dfy"
 include "Util.dfy"
-include "Laws.dfy"
+include "CorrectnessSSA.dfy"
 
 class VariablesSSA {
 
@@ -705,102 +705,6 @@ method {:verify false}OrganizeVariables(vars1: seq<Variable>, vars2: seq<Variabl
 	}
 }*/
 
-function InstancesAndVariablesBreakdown(S: Statement, X: seq<Variable>, 
-	liveOnEntry: set<Variable>, liveOnExit: set<Variable>, XLs: set<Variable>, vsSSA: VariablesSSA): 
-	(seq<Variable>,seq<Variable>,seq<Variable>,seq<Variable>,seq<Variable>,seq<Variable>,
-	seq<Variable>,seq<Variable>,seq<Variable>,seq<Variable>,seq<Variable>)
-/*	requires ValidVsSSA(vsSSA)
-	reads vsSSA
-{
-	var XL3iSet := liveOnEntry * liveOnExit;
-	assert XL3i <= liveOnEntry && XL3i <= liveOnExitX;
-	var XL3i := setToSeq(XL3i);
-	var X3 := vsSSA.instancesToVariables(XL3i);
-	var X3Set := setOf(X3);
-
-	var XL1iXL2iXL4i := liveOnEntry - XL3iSet;
-	assert XL1iXL2iXL4i <= liveOnEntry;
-	var temp := setToSeq(XL1iXL2iXL4i);
-	var X1X2X4 := vsSSA.instancesToVariables(temp);
-	var XL4fXL5f := liveOnExitX - XL3i;
-	assert XL4fXL5f <= liveOnExitX;
-	var temp2 := setToSeq(XL4fXL5f);
-	var X4X5 := vsSSA.instancesToVariables(temp2);
-	var X4Set := setOf(X1X2X4) * setOf(X4X5) * setOf(X);
-	//var X4 := vsSSA.instancesToVariables(X4Set)
-	var X5Set := setOf(X4X5) - X4Set;
-	var X5 := setToSeq(X5Set);
-	var XL5f := vsSSA.getInstancesOfVaribleSeq
-	
-	var X1X2 := setOf(X1X2X4) - X4;
-	var X2 := X1X2 * def(Assignment(LHS,RHS));
-	var X1 := X1X2 - X2;
-
-	(XL1i,XL2i,XL3i,XL4i,XL4f,XL5f,X1,X2,X3,X4,X5)
-}*/
-
-function ToSSALeft(S: Statement, XL3i: seq<Variable>, XL4f: seq<Variable>, XL5f: seq<Variable>, 
-	X3: seq<Variable>, X4: seq<Variable>, X5: seq<Variable>, Y: seq<Variable>): Statement
-{
-	Live(XL3i+XL4f+XL5f+Y,SeqComp(S,Assignment(XL3i+XL4f+XL5f,seqVarToSeqExpr(X3+X4+X5))))
-}
-
-function ToSSARight(XL1i: seq<Variable>, XL2i: seq<Variable>, XL3i: seq<Variable>, XL4i: seq<Variable>,	
-	X1: seq<Variable>, X2: seq<Variable>, X3: seq<Variable>, X4: seq<Variable>, 
-	S': Statement, XL4f: seq<Variable>, XL5f: seq<Variable>, Y: seq<Variable>): Statement
-{
-	Live(XL3i+XL4f+XL5f+Y,SeqComp(Assignment(XL1i+XL2i+XL3i+XL4i,seqVarToSeqExpr(X1+X2+X3+X4)),S'))
-}
-
-// TODO: move to a more central/reusable location: Util? Definitions?
-predicate mutuallyDisjoint3<T>(s1: seq<T>, s2: seq<T>, s3: seq<T>)
-{
-	|setOf(s1+s2+s3)| == |s1|+|s2|+|s3|
-}
-
-predicate mutuallyDisjoint4<T>(s1: seq<T>, s2: seq<T>, s3: seq<T>, s4: seq<T>)
-{
-	|setOf(s1+s2+s3+s4)| == |s1|+|s2|+|s3|+|s4|
-}
-
-predicate mutuallyDisjoint5<T>(s1: seq<T>, s2: seq<T>, s3: seq<T>, s4: seq<T>, s5: seq<T>)
-{
-	|setOf(s1+s2+s3+s4+s5)| == |s1|+|s2|+|s3|+|s4|+|s5|
-}
-
-predicate mutuallyDisjoint6<T>(s1: seq<T>, s2: seq<T>, s3: seq<T>, s4: seq<T>, s5: seq<T>, s6: seq<T>)
-{
-	|setOf(s1+s2+s3+s4+s5+s6)| == |s1|+|s2|+|s3|+|s4|+|s5|+|s6|
-}
-
-predicate PreconditionsOfToSSA(S: Statement, S': Statement, X: seq<Variable>, 
-	XL1i: seq<Variable>, XL2i: seq<Variable>, XL3i: seq<Variable>, XL4i: seq<Variable>, 
-	XL4f: seq<Variable>, XL5f: seq<Variable>, 
-	X1: seq<Variable>, X2: seq<Variable>, X3: seq<Variable>, X4: seq<Variable>, X5: seq<Variable>, 
-	Y: set<Variable>, XLs: set<Variable>)
-{
-	glob(S) <= setOf(X)+Y                                                                                    // P1
-	&& mutuallyDisjoint5(X1,X2,X3,X4,X5) && setOf(X1+X2+X3+X4+X5) <= setOf(X)                                // P2
-	&& mutuallyDisjoint6(XL1i,XL2i,XL3i,XL4i,XL4f,XL5f) && setOf(XL1i+XL2i+XL3i+XL4i+XL4f+XL5f) <= XLs       // P3
-	&& setOf(X) !! Y && XLs !! setOf(X)+Y                                                                    // P4
-	&& setOf(X1) !! setOf(X3) && setOf(X1+X3) !! def(S)                                                      // P5
-	&& mutuallyDisjoint3(X2,X4,X5) && setOf(X2+X4+X5) <= def(S)                                              // P6
-	&& mutuallyDisjoint4(X1,X2,X3,X4) && setOf(X) * (setOf(X3+X4+X5)-ddef(S)+input(S)) <= setOf(X1+X2+X3+X4) // P7
-}
-
-predicate CorrectnessOfToSSA(S: Statement, S': Statement, X: seq<Variable>, liveOnEntryX: set<Variable>, liveOnExitX: set<Variable>, Y: set<Variable>, XLs: set<Variable>, vsSSA: VariablesSSA)
-	reads * //vsSSA
-	requires ValidVsSSA(vsSSA)
-{
-	var xs := InstancesAndVariablesBreakdown(S,X,liveOnEntryX,liveOnExitX,XLs,vsSSA);
-	var XL1i,XL2i,XL3i,XL4i,XL4f,XL5f,X1,X2,X3,X4,X5 := xs.0,xs.1,xs.2,xs.3,xs.4,xs.5,xs.6,xs.7,xs.8,xs.9,xs.10;
-	var Y' := fSetToSeq(Y);
-	PreconditionsOfToSSA(S,S',X,XL1i,XL2i,XL3i,XL4i,XL4f,XL5f,X1,X2,X3,X4,X5,Y,XLs) ==>
-	Valid(ToSSALeft(S,XL3i,XL4f,XL5f,X3,X4,X5,Y')) && Valid(ToSSARight(XL1i,XL2i,XL3i,XL4i,X1,X2,X3,X4,S',XL4f,XL5f,Y')) &&
-	EquivalentStatments(ToSSALeft(S,XL3i,XL4f,XL5f,X3,X4,X5,Y'),ToSSARight(XL1i,XL2i,XL3i,XL4i,X1,X2,X3,X4,S',XL4f,XL5f,Y')) // Q1
-	&& setOf(X) !! glob(S') // Q2
-}
-
 method ToSSA(S: Statement, X: seq<Variable>, liveOnEntryX: set<Variable>, liveOnExitX: set<Variable>, Y: set<Variable>, XLs: set<Variable>, vsSSA: VariablesSSA) returns(S': Statement)
 	requires Valid(S)
 	requires (Core(S))
@@ -1129,7 +1033,7 @@ method {:verify false}IfToSSA(B : BooleanExpression, S1 : Statement, S2 : Statem
 	ensures forall v :: v in X ==> vsSSA.existsInstance(v)
 	ensures forall v :: v in Y ==> vsSSA.existsInstance(v)
 	ensures forall v :: v in old(vsSSA.instancesOf) ==> v in vsSSA.instancesOf && (forall i :: i in old(vsSSA.instancesOf[v]) ==> i in vsSSA.instancesOf[v])
-	ensures CorrectnessOfToSSA(IF(B,S1,S2),S',X,liveOnEntryX,liveOnExitX,Y,XLs,vsSSA)
+	//ensures CorrectnessOfToSSA(IF(B,S1,S2),S',X1,X2,X3,X4,X5,XL1i,XL2i,XL3i,XL4i,XL4f,XL5f,Y,XLs)
 {
 	// defined in thesis:
 	// toSSA.(IF ,X, (XL1i, XL2i, XL3i, XL4i), (XL3i, XL4f, XL5f), Y, XLs) is:
@@ -1299,9 +1203,10 @@ method {:verify false}IfToSSA(B : BooleanExpression, S1 : Statement, S2 : Statem
 	S' := IF(B', tempSeqComp1, tempSeqComp2);
 	//S' := IF(B', SeqComp(S1', Assignment(XL4fSeqThen + XL5fSeq, XL4t + XL5t)), SeqComp(S2', Assignment(XL4fSeqElse + XL5fSeq, XL4e + XL5e)));
 	assert Valid(S');
-	assert CorrectnessOfToSSA(IF(B,S1,S2),S',X,liveOnEntryX,liveOnExitX,Y,XLs,vsSSA) by
+/*
+	assert CorrectnessOfToSSA(IF(B,S1,S2),S',X1,X2,X3,X4,X5,XL1i,XL2i,XL3i,XL4i,XL4f,XL5f,Y,XLs) by
 	{
-		assume CorrectnessOfToSSA(IF(B,S1,S2),S',X,XL1i+XL2i+XL3i+XL4i,XL3i+XL4f+XL5f,Y,XLs,vsSSA);
+		assume CorrectnessOfToSSA(IF(B,S1,S2),S',X1,X2,X3,X4,X5,XL1i,XL2i,XL3i,XL4i,XL4f,XL5f,Y,XLs,vsSSA);
 /*		
 		var S1' := tempSeqComp1;
 		assert CorrectnessOfToSSA(IF(B,S1,S2),S',X,XL1i+XL2i+XL3i+XL4i,XL3i+XL4f+XL5f,Y,XLs,vsSSA) by
@@ -1312,78 +1217,8 @@ method {:verify false}IfToSSA(B : BooleanExpression, S1 : Statement, S2 : Statem
 		}*/
 		assert liveOnEntryX == XL1i+XL2i+XL3i+XL4i;
 		assert liveOnExitX == XL3i+XL4f+XL5f;
-	}
+	}*/
 }
-
-lemma LemmaIfToSSAIsCorrect(B: BooleanExpression, S1: Statement, S2: Statement,
-		X: seq<Variable>, XL1i: seq<Variable>, XL2i: seq<Variable>, XL3i: seq<Variable>, XL4i: seq<Variable>,
-		XL4f: seq<Variable>, XL5f: seq<Variable>, Y: seq<Variable>, XLs: set<Variable>,
-		X1: seq<Variable>, X2: seq<Variable>, X3: seq<Variable>, X4: seq<Variable>, X5: seq<Variable>,
-		S1': Statement,	XL4t: seq<Variable>, XL5t: seq<Variable>, XL4e: seq<Variable>, XL5e: seq<Variable>,
-		X4d1: seq<Variable>, X4d2: seq<Variable>, X4d1d2: seq<Variable>,
-		XL4d1t: seq<Variable>, XL4d1e: seq<Variable>, XL4d1d2t: seq<Variable>, XL4d1d2e: seq<Variable>, XL4d2i: seq<Variable>,
-		XL4d1i: seq<Variable>, XL4d2e: seq<Variable>, XLs': set<Variable>, XLs'': set<Variable>,
-		S2': Statement, vsSSA: VariablesSSA)
-	requires ValidVsSSA(vsSSA)
-	requires |X1+X2+X3+X4| == |XL1i+XL2i+XL3i+XL4i| && setOf(X1+X2+X3+X4) !! setOf(XL1i+XL2i+XL3i+XL4i)
-	requires var B' := BSubstitute(B,X1+X2+X3+X4,XL1i+XL2i+XL3i+XL4i);
-		PreconditionsOfToSSA(IF(B,S1,S2),IF(B',S1',S2'),X,XL1i,XL2i,XL3i,XL4i,XL4f,XL5f,X1,X2,X3,X4,X5,setOf(Y),XLs) &&
-		Valid(ToSSALeft(IF(B,S1,S2),XL3i,XL4f,XL5f,X3,X4,X5,Y)) &&
-		Valid(ToSSARight(XL1i,XL2i,XL3i,XL4i,X1,X2,X3,X4,IF(B',S1',S2'),XL4f,XL5f,Y))
-	ensures var B' := BSubstitute(B,X1+X2+X3+X4,XL1i+XL2i+XL3i+XL4i);
-		CorrectnessOfToSSA(IF(B,S1,S2),IF(B',S1',S2'),X,setOf(XL1i+XL2i+XL3i+XL4i),setOf(XL3i+XL4f+XL5f),setOf(Y),XLs,vsSSA)
-/*{
-	var B' := BSubstitute(B,X1+X2+X3+X4,XL1i+XL2i+XL3i+XL4i);
-	var S,S' := IF(B,S1,S2),IF(B',S1',S2');
-	// TODO: Be sure first that the breakdown is the same; is it???
-	var liveOnEntryX,liveOnExitX := setOf(XL1i+XL2i+XL3i+XL4i),setOf(XL3i+XL4f+XL5f);
-	var xs := InstancesAndVariablesBreakdown(S,X,liveOnEntryX,liveOnExitX,XLs,vsSSA);
-	var XL1i',XL2i',XL3i',XL4i',XL4f',XL5f',X1',X2',X3',X4',X5' := xs.0,xs.1,xs.2,xs.3,xs.4,xs.5,xs.6,xs.7,xs.8,xs.9,xs.10;
-	//and then...
-	assume Valid(ToSSALeft(S,XL3i',XL4f',XL5f',X3',X4',X5',Y)) && Valid(ToSSARight(XL1i,XL2i,XL3i,XL4i,X1,X2,X3,X4,S',XL4f,XL5f,Y)) &&
-		EquivalentStatments(ToSSALeft(S,XL3i,XL4f,XL5f,X3,X4,X5,Y),ToSSARight(XL1i,XL2i,XL3i,XL4i,X1,X2,X3,X4,S',XL4f,XL5f,Y));// by {
-}/
-/*
-/*	
-not sure about the parameters to D3, should figure it out and fix; and then
-should show that the preconditions above indeed guarantee that the preconditions of D3 (below, after the appropriate parameter substitutions) all hold;
-and finally show that the postcondition of D3 (again, with the appropriate substitution) guarantee that our postconditions hold.
-
-D.3:
-	Live(XL2f+Y,SeqComp(IF(B,S1,S2),Assignment(XL2f,seqVarToSeqExpr(X2))))
-==
-	Live(XL2f+Y,SeqComp(Assignment(XL1i,seqVarToSeqExpr(X1)),IF(B',S1',S2')))
-
-
-*/
-		var XL1i',XL2f',X1',X2' := setOf(XL1i+XL2i+XL3i+XL4i),X1+X2+X3+X4,
-		assert TransformationD3Left(B,S1,S2,X2,XL2f,Y),TransformationD3Right(B',S1',S2',X1,XL1i,XL2f,Y) && 
-			EquivalentStatments(TransformationD3Left(B,S1,S2,X2,XL2f,Y),TransformationD3Right(B',S1',S2',X1,XL1i,XL2f,Y)) by {
-		TransformationD3(B,B',S1,S2,S1',S2',X1,X2,XL1i,XL2i,XL2f,Y);
-
-/*
-requires Valid(Live(XL2f+Y,SeqComp(S2,Assignment(XL2f,seqVarToSeqExpr(X2)))))
-	requires Valid(Live(XL2f+Y,SeqComp(Assignment(XL1i,seqVarToSeqExpr(X1)),S2')))
-	requires EquivalentStatments(Live(XL2f+Y,SeqComp(S2,Assignment(XL2f,seqVarToSeqExpr(X2)))),
-		Live(XL2f+Y,SeqComp(Assignment(XL1i,seqVarToSeqExpr(X1)),S2'))) // P5
-	requires Valid(Live(XL2f+Y,SeqComp(S1,Assignment(XL2f,seqVarToSeqExpr(X2)))))
-	requires Valid(Live(XL2f+Y,SeqComp(Assignment(XL1i,seqVarToSeqExpr(X1)),S1')))
-	requires EquivalentStatments(Live(XL2f+Y,SeqComp(S1,Assignment(XL2f,seqVarToSeqExpr(X2)))),
-		Live(XL2f+Y,SeqComp(Assignment(XL1i,seqVarToSeqExpr(X1)),S1'))) // P4
-	requires setOf(XL1i) !! B.1 // P3
-	requires setOf(XL1i) !! setOf(X1) // P2
-	requires |X1| == |XL1i|
-	requires EquivalentBooleanExpressions(B',BSubstitute(B,X1,XL1i)) // P1
-
-	requires Valid(TransformationD3Left(B,S1,S2,X2,XL2f,Y))
-	requires Valid(TransformationD3Right(B',S1',S2',X1,XL1i,XL2f,Y))
-	ensures EquivalentStatments(TransformationD3Left(B,S1,S2,X2,XL2f,Y),
-			TransformationD3Right(B',S1',S2',X1,XL1i,XL2f,Y))
-			*/
-	}	
-	assert setOf(X) !! glob(S'); // Q2
-}*/
-*/
 
 method {:verify false}DoToSSA(B : BooleanExpression, S : Statement, X: seq<Variable>, liveOnEntryX: set<Variable>, liveOnExitX: set<Variable>, Y: set<Variable>, XLs: set<Variable>, vsSSA: VariablesSSA) returns (S'': Statement)
 	requires Valid(DO(B, S))
@@ -1716,137 +1551,3 @@ method {:verify false}DoFromSSA(B' : BooleanExpression, S' : Statement, XLs: set
 	S := MergeVars(S', XLs, X, XLi, XLi, Y, vsSSA);
 	S := DO(B, S);
 }
-
-function TransformationD3Left(B: BooleanExpression, 
-		S1: Statement, S2: Statement,
-		X2: seq<Variable>,
-		XL2f: seq<Variable>, Y: seq<Variable>): Statement
-{
-	Live(XL2f+Y,SeqComp(IF(B,S1,S2),Assignment(XL2f,seqVarToSeqExpr(X2))))
-}
-
-function TransformationD3Right(B': BooleanExpression, 
-		S1': Statement, S2': Statement,
-		X1: seq<Variable>,
-		XL1i: seq<Variable>, XL2f: seq<Variable>, Y: seq<Variable>): Statement
-{
-	Live(XL2f+Y,SeqComp(Assignment(XL1i,seqVarToSeqExpr(X1)),IF(B',S1',S2')))
-}
-
-lemma TransformationD3(B: BooleanExpression, B': BooleanExpression, 
-		S1: Statement, S2: Statement, S1': Statement, S2': Statement,
-		X1: seq<Variable>, X2: seq<Variable>,
-		XL1i: seq<Variable>, XL2i: seq<Variable>, XL2f: seq<Variable>, Y: seq<Variable>)
-	requires Valid(Live(XL2f+Y,SeqComp(S2,Assignment(XL2f,seqVarToSeqExpr(X2)))))
-	requires Valid(Live(XL2f+Y,SeqComp(Assignment(XL1i,seqVarToSeqExpr(X1)),S2')))
-	requires EquivalentStatments(Live(XL2f+Y,SeqComp(S2,Assignment(XL2f,seqVarToSeqExpr(X2)))),
-		Live(XL2f+Y,SeqComp(Assignment(XL1i,seqVarToSeqExpr(X1)),S2'))) // P5
-	requires Valid(Live(XL2f+Y,SeqComp(S1,Assignment(XL2f,seqVarToSeqExpr(X2)))))
-	requires Valid(Live(XL2f+Y,SeqComp(Assignment(XL1i,seqVarToSeqExpr(X1)),S1')))
-	requires EquivalentStatments(Live(XL2f+Y,SeqComp(S1,Assignment(XL2f,seqVarToSeqExpr(X2)))),
-		Live(XL2f+Y,SeqComp(Assignment(XL1i,seqVarToSeqExpr(X1)),S1'))) // P4
-	requires setOf(XL1i) !! B.1 // P3
-	requires setOf(XL1i) !! setOf(X1) // P2
-	requires |X1| == |XL1i|
-	requires EquivalentBooleanExpressions(B',BSubstitute(B,X1,XL1i)) // P1
-
-	requires Valid(TransformationD3Left(B,S1,S2,X2,XL2f,Y))
-	requires Valid(TransformationD3Right(B',S1',S2',X1,XL1i,XL2f,Y))
-	ensures EquivalentStatments(TransformationD3Left(B,S1,S2,X2,XL2f,Y),
-			TransformationD3Right(B',S1',S2',X1,XL1i,XL2f,Y))
-{
-	var T1 := TransformationD3Left(B,S1,S2,X2,XL2f,Y);
-	var T2 := TransformationD3Right(B',S1',S2',X1,XL1i,XL2f,Y);
-	forall P: Predicate ensures EquivalentPredicates(wp(T1,P),wp(T2,P)) {
-		var P1 := wp(T1,P);
-		var P2 := wp(T2,P);
-		forall s: State | P1.0.requires(s) && P2.0.requires(s) ensures P1.0(s) == P2.0(s) {
-			calc {
-				wp(T2,P).0(s);
-			== // def. of T2 and of TransformationD3Right
-				wp(Live(XL2f+Y,SeqComp(Assignment(XL1i,seqVarToSeqExpr(X1)),IF(B',S1',S2'))),P).0(s);
-			== { assert B'.0(s) == BSubstitute(B,X1,XL1i).0(s); // from P1
-						var IF1,IF1',V := IF(BSubstitute(B,X1,XL1i),S1',S2'),IF(B',S1',S2'),XL2f+Y;
-						assert EquivalentStatments(IF1',IF1);
-						var A1 := Assignment(XL1i,seqVarToSeqExpr(X1));
-						var SC1,SC1' := SeqComp(A1,IF1),SeqComp(A1,IF1');
-						assert EquivalentStatments(SC1',SC1) by { assert EquivalentStatments(IF1',IF1); Leibniz4(A1,IF1,IF1'); }
-						assert EquivalentStatments(Live(V,SC1'),Live(V,SC1));
-						}
-				wp(Live(XL2f+Y,SeqComp(Assignment(XL1i,seqVarToSeqExpr(X1)),IF(BSubstitute(B,X1,XL1i),S1',S2'))),P).0(s);
-			== { assert setOf(XL1i) !! setOf(X1); // P2
-						Law18b(S1',S2',BSubstitute(B,X1,XL1i),[],XL1i,[],seqVarToSeqExpr(X1)); }
-				wp(Live(XL2f+Y,SeqComp(Assignment(XL1i,seqVarToSeqExpr(X1)),IF(BSubstituteVbyE(BSubstitute(B,X1,XL1i),XL1i,seqVarToSeqExpr(X1)),S1',S2'))),P).0(s);
-			== {// remove redundant (reversed) double sub.
-					var B'' := BSubstituteVbyE(BSubstitute(B,X1,XL1i),XL1i,seqVarToSeqExpr(X1));
-					assert EquivalentBooleanExpressions(B,B'') by { assert setOf(XL1i) !! B.1; /* P3 */ ReversedDoubleSubstitutions(B,X1,XL1i); }
-					assert EquivalentStatments(IF(B,S1',S2'),IF(B'',S1',S2'));
-					var A1,IF1,IF1',V := Assignment(XL1i,seqVarToSeqExpr(X1)),IF(B,S1',S2'),IF(B'',S1',S2'),XL2f+Y;
-					var SC1,SC2 := SeqComp(A1,IF1'),SeqComp(A1,IF1);
-					assert EquivalentStatments(SC1,SC2) by { assert EquivalentStatments(IF1',IF1); Leibniz4(A1,IF1',IF1); }
-					assert EquivalentStatments(Live(V,SC1),Live(V,SC2));
-					}
-				wp(Live(XL2f+Y,SeqComp(Assignment(XL1i,seqVarToSeqExpr(X1)),IF(B,S1',S2'))),P).0(s);
-			== { assert setOf(XL1i) !! B.1; // P3
-						Law3(Assignment(XL1i,seqVarToSeqExpr(X1)),S1',S2',B); } // distribute statement over IF
-				wp(Live(XL2f+Y,IF(B,SeqComp(Assignment(XL1i,seqVarToSeqExpr(X1)),S1'),SeqComp(Assignment(XL1i,seqVarToSeqExpr(X1)),S2'))),P).0(s);
-			== { Law21(B,SeqComp(Assignment(XL1i,seqVarToSeqExpr(X1)),S1'),SeqComp(Assignment(XL1i,seqVarToSeqExpr(X1)),S2'),XL2f+Y); } // propagate liveness info.
-				wp(Live(XL2f+Y,IF(B,Live(XL2f+Y,SeqComp(Assignment(XL1i,seqVarToSeqExpr(X1)),S1')),
-					Live(XL2f+Y,SeqComp(Assignment(XL1i,seqVarToSeqExpr(X1)),S2')))),P).0(s);
-			== { var V := XL2f+Y;
-						var T1 := Live(V,SeqComp(S1,Assignment(XL2f,seqVarToSeqExpr(X2))));
-						var T1' := Live(V,SeqComp(Assignment(XL1i,seqVarToSeqExpr(X1)),S1'));
-						assert EquivalentStatments(T1,T1'); // P4
-						var T2 := Live(V,SeqComp(S2,Assignment(XL2f,seqVarToSeqExpr(X2))));
-						var T2' := Live(V,SeqComp(Assignment(XL1i,seqVarToSeqExpr(X1)),S2'));
-						assert EquivalentStatments(T2,T2'); // P5
-						var IF1,IF1' := IF(B,T1,T2),IF(B,T1',T2');
-						assert EquivalentStatments(IF1',IF1);
-						assert EquivalentStatments(Live(V,IF1'),Live(V,IF1));
-					}
-				wp(Live(XL2f+Y,IF(B,Live(XL2f+Y,SeqComp(S1,Assignment(XL2f,seqVarToSeqExpr(X2)))),
-					Live(XL2f+Y,SeqComp(S2,Assignment(XL2f,seqVarToSeqExpr(X2)))))),P).0(s);
-			== { Law21(B,SeqComp(S1,Assignment(XL2f,seqVarToSeqExpr(X2))),SeqComp(S2,Assignment(XL2f,seqVarToSeqExpr(X2))),XL2f+Y); } // remove liveness info.
-				wp(Live(XL2f+Y,IF(B,SeqComp(S1,Assignment(XL2f,seqVarToSeqExpr(X2))),SeqComp(S2,Assignment(XL2f,seqVarToSeqExpr(X2))))),P).0(s);
-			== { Law4(S1,S2,Assignment(XL2f,seqVarToSeqExpr(X2)),B); } // dist. IF over ";"
-				wp(Live(XL2f+Y,SeqComp(IF(B,S1,S2),Assignment(XL2f,seqVarToSeqExpr(X2)))),P).0(s);
-			== // def. of T1 and of TransformationD3Left
-				wp(T1,P).0(s);
-			}
-		}
-	}
-}
-
-//method TransformationD5(S: Statement, X: seq<Variable>, X: seq<Variable>) returns (S': Statement)
-
-function IfToSSACorrectnessLeft(B: BooleanExpression, S1: Statement, S2: Statement,
-		X3: seq<Variable>, X4: seq<Variable>, X5: seq<Variable>, // live-on-exit variables (the X2 of D.3)
-		XL3i: seq<Variable>, XL4f: seq<Variable>, XL5f: seq<Variable>, // live-on-exit instances (the XL2f of D.3)
-		Y: seq<Variable>): Statement
-{
-//	Live(XL3i+XL4f+XL5f+Y,SeqComp(IF(B,S1,S2),Assignment(XL3i+XL4f+XL5f,seqVarToSeqExpr(X3+X4+X5))))
-	TransformationD3Left(B,S1,S2,X3+X4+X5,XL3i+XL4f+XL5f,Y)
-//	Live(XL2f          +Y,SeqComp(IF(B,S1,S2),Assignment(XL2f          ,seqVarToSeqExpr(X2      ))))
-}
-
-function IfToSSACorrectnessRight(B': BooleanExpression, S1': Statement, S2': Statement,
-		X1: seq<Variable>, X2: seq<Variable>, X3: seq<Variable>, X4: seq<Variable>, // live-on-entry variables (the X1 of D.3)
-		XL1i: seq<Variable>, XL2i: seq<Variable>, XL3i: seq<Variable>, XL4i: seq<Variable>, // live-on-entry instances (the XL1i of D.3)
-		XL4f: seq<Variable>, XL5f: seq<Variable>, // along with XL1i: live-on-exit instances (the XL2f of D.3)
-		Y: seq<Variable>): Statement
-{
-//	Live(XL3i+XL4f+XL5f+Y,SeqComp(Assignment(XL1i+XL2i+XL3i+XL4i,seqVarToSeqExpr(X1+X2+X3+X4)),IF(B',S1',S2')))
-	TransformationD3Right(B',S1',S2',X1+X2+X3+X4,XL1i+XL2i+XL3i+XL4i,XL3i+XL4f+XL5f,Y)
-//	Live(XL2f          +Y,SeqComp(Assignment(XL1i               ,seqVarToSeqExpr(X1         )),IF(B',S1',S2')))
-}
-
-lemma IfToSSACorrectness(B: BooleanExpression, S1: Statement, S2: Statement, B': BooleanExpression, S1': Statement, S2': Statement,
-		X1: seq<Variable>, X2: seq<Variable>, X3: seq<Variable>, X4: seq<Variable>, // live-on-entry variables (the X1 of D.3)
-		X5: seq<Variable>, // along with X3,X4: live-on-exit variables (the X2 of D.3)
-		XL1i: seq<Variable>, XL2i: seq<Variable>, XL3i: seq<Variable>, XL4i: seq<Variable>, // live-on-entry instances (the XL1i of D.3)
-		XL4f: seq<Variable>, XL5f: seq<Variable>, // along with XL1i: live-on-exit instances (the XL2f of D.3)
-		Y: seq<Variable>)
-	requires Valid(IfToSSACorrectnessLeft(B,S1,S2,X3,X4,X5,XL3i,XL4f,XL5f,Y))
-	requires Valid(IfToSSACorrectnessRight(B',S1',S2',X1,X2,X3,X4,XL1i,XL2i,XL3i,XL4i,XL4f,XL5f,Y))
-	ensures EquivalentStatments(IfToSSACorrectnessLeft(B,S1,S2,X3,X4,X5,XL3i,XL4f,XL5f,Y),
-			IfToSSACorrectnessRight(B',S1',S2',X1,X2,X3,X4,XL1i,XL2i,XL3i,XL4i,XL4f,XL5f,Y))
