CorrectnessSSA.dfy
@@ -1,0 +1,269 @@
+include "Definitions.dfy"
+include "Substitutions.dfy"
+include "Util.dfy"
+include "Laws.dfy"
+
+function ToSSALeft(S: Statement, XL3i: seq<Variable>, XL4f: seq<Variable>, XL5f: seq<Variable>, 
+	X3: seq<Variable>, X4: seq<Variable>, X5: seq<Variable>, Y: seq<Variable>): Statement
+{
+	Live(XL3i+XL4f+XL5f+Y,SeqComp(S,Assignment(XL3i+XL4f+XL5f,seqVarToSeqExpr(X3+X4+X5))))
+}
+
+function ToSSARight(XL1i: seq<Variable>, XL2i: seq<Variable>, XL3i: seq<Variable>, XL4i: seq<Variable>,	
+	X1: seq<Variable>, X2: seq<Variable>, X3: seq<Variable>, X4: seq<Variable>, 
+	S': Statement, XL4f: seq<Variable>, XL5f: seq<Variable>, Y: seq<Variable>): Statement
+{
+	Live(XL3i+XL4f+XL5f+Y,SeqComp(Assignment(XL1i+XL2i+XL3i+XL4i,seqVarToSeqExpr(X1+X2+X3+X4)),S'))
+}
+
+// TODO: move to a more central/reusable location: Util? Definitions?
+predicate mutuallyDisjoint3<T>(s1: seq<T>, s2: seq<T>, s3: seq<T>)
+{
+	|setOf(s1+s2+s3)| == |s1|+|s2|+|s3|
+}
+
+predicate mutuallyDisjoint4<T>(s1: seq<T>, s2: seq<T>, s3: seq<T>, s4: seq<T>)
+{
+	|setOf(s1+s2+s3+s4)| == |s1|+|s2|+|s3|+|s4|
+}
+
+predicate mutuallyDisjoint5<T>(s1: seq<T>, s2: seq<T>, s3: seq<T>, s4: seq<T>, s5: seq<T>)
+{
+	|setOf(s1+s2+s3+s4+s5)| == |s1|+|s2|+|s3|+|s4|+|s5|
+}
+
+predicate mutuallyDisjoint6<T>(s1: seq<T>, s2: seq<T>, s3: seq<T>, s4: seq<T>, s5: seq<T>, s6: seq<T>)
+{
+	|setOf(s1+s2+s3+s4+s5+s6)| == |s1|+|s2|+|s3|+|s4|+|s5|+|s6|
+}
+
+predicate PreconditionsOfToSSA(S: Statement, S': Statement, X: seq<Variable>, 
+	XL1i: seq<Variable>, XL2i: seq<Variable>, XL3i: seq<Variable>, XL4i: seq<Variable>, 
+	XL4f: seq<Variable>, XL5f: seq<Variable>, 
+	X1: seq<Variable>, X2: seq<Variable>, X3: seq<Variable>, X4: seq<Variable>, X5: seq<Variable>, 
+	Y: seq<Variable>, XLs: set<Variable>)
+{
+	glob(S) <= setOf(X+Y)                                                                                    // P1
+	&& mutuallyDisjoint5(X1,X2,X3,X4,X5) && setOf(X1+X2+X3+X4+X5) <= setOf(X)                                // P2
+	&& mutuallyDisjoint6(XL1i,XL2i,XL3i,XL4i,XL4f,XL5f) && setOf(XL1i+XL2i+XL3i+XL4i+XL4f+XL5f) <= XLs       // P3
+	&& setOf(X) !! setOf(Y) && XLs !! setOf(X+Y)                                                             // P4
+	&& setOf(X1) !! setOf(X3) && setOf(X1+X3) !! def(S)                                                      // P5
+	&& mutuallyDisjoint3(X2,X4,X5) && setOf(X2+X4+X5) <= def(S)                                              // P6
+	&& mutuallyDisjoint4(X1,X2,X3,X4) && setOf(X) * (setOf(X3+X4+X5)-ddef(S)+input(S)) <= setOf(X1+X2+X3+X4) // P7
+}
+
+predicate CorrectnessOfToSSA(S: Statement, S': Statement,
+	X1: seq<Variable>, X2: seq<Variable>, X3: seq<Variable>, X4: seq<Variable>, X5: seq<Variable>,
+	XL1i: seq<Variable>, XL2i: seq<Variable>, XL3i: seq<Variable>, XL4i: seq<Variable>,
+	XL4f: seq<Variable>, XL5f: seq<Variable>, Y: seq<Variable>, XLs: set<Variable>)
+	reads *
+{
+	var X := X1+X2+X3+X4+X5;
+	PreconditionsOfToSSA(S,S',X,XL1i,XL2i,XL3i,XL4i,XL4f,XL5f,X1,X2,X3,X4,X5,Y,XLs) ==>
+	Valid(ToSSALeft(S,XL3i,XL4f,XL5f,X3,X4,X5,Y)) && Valid(ToSSARight(XL1i,XL2i,XL3i,XL4i,X1,X2,X3,X4,S',XL4f,XL5f,Y)) &&
+	EquivalentStatments(ToSSALeft(S,XL3i,XL4f,XL5f,X3,X4,X5,Y),ToSSARight(XL1i,XL2i,XL3i,XL4i,X1,X2,X3,X4,S',XL4f,XL5f,Y)) // Q1
+	&& setOf(X) !! glob(S') // Q2
+}
+
+lemma LemmaIfToSSAIsCorrect(B: BooleanExpression, S1: Statement, S2: Statement,
+		X: seq<Variable>, XL1i: seq<Variable>, XL2i: seq<Variable>, XL3i: seq<Variable>, XL4i: seq<Variable>,
+		XL4f: seq<Variable>, XL5f: seq<Variable>, Y: seq<Variable>, XLs: set<Variable>,
+		X1: seq<Variable>, X2: seq<Variable>, X3: seq<Variable>, X4: seq<Variable>, X5: seq<Variable>,
+		S1': Statement,	XL4t: seq<Variable>, XL5t: seq<Variable>, XL4e: seq<Variable>, XL5e: seq<Variable>,
+		X4d1: seq<Variable>, X4d2: seq<Variable>, X4d1d2: seq<Variable>,
+		XL4d1t: seq<Variable>, XL4d1e: seq<Variable>, XL4d1d2t: seq<Variable>, XL4d1d2e: seq<Variable>, XL4d2i: seq<Variable>,
+		XL4d1i: seq<Variable>, XL4d2e: seq<Variable>, XLs': set<Variable>, XLs'': set<Variable>,
+		S2': Statement)
+	requires |X1+X2+X3+X4| == |XL1i+XL2i+XL3i+XL4i| && setOf(X1+X2+X3+X4) !! setOf(XL1i+XL2i+XL3i+XL4i)
+	requires var B' := BSubstitute(B,X1+X2+X3+X4,XL1i+XL2i+XL3i+XL4i);
+		PreconditionsOfToSSA(IF(B,S1,S2),IF(B',S1',S2'),X,XL1i,XL2i,XL3i,XL4i,XL4f,XL5f,X1,X2,X3,X4,X5,Y,XLs) &&
+		Valid(ToSSALeft(IF(B,S1,S2),XL3i,XL4f,XL5f,X3,X4,X5,Y)) &&
+		Valid(ToSSARight(XL1i,XL2i,XL3i,XL4i,X1,X2,X3,X4,IF(B',S1',S2'),XL4f,XL5f,Y))
+	ensures var B' := BSubstitute(B,X1+X2+X3+X4,XL1i+XL2i+XL3i+XL4i);
+		CorrectnessOfToSSA(IF(B,S1,S2),IF(B',S1',S2'),X1,X2,X3,X4,X5,XL1i,XL2i,XL3i,XL4i,XL4f,XL5f,Y,XLs)
+/*{
+	var B' := BSubstitute(B,X1+X2+X3+X4,XL1i+XL2i+XL3i+XL4i);
+	var S,S' := IF(B,S1,S2),IF(B',S1',S2');
+	// TODO: Be sure first that the breakdown is the same; is it???
+	var liveOnEntryX,liveOnExitX := setOf(XL1i+XL2i+XL3i+XL4i),setOf(XL3i+XL4f+XL5f);
+	var xs := InstancesAndVariablesBreakdown(S,X,liveOnEntryX,liveOnExitX,XLs,vsSSA);
+	var XL1i',XL2i',XL3i',XL4i',XL4f',XL5f',X1',X2',X3',X4',X5' := xs.0,xs.1,xs.2,xs.3,xs.4,xs.5,xs.6,xs.7,xs.8,xs.9,xs.10;
+	//and then...
+	assume Valid(ToSSALeft(S,XL3i',XL4f',XL5f',X3',X4',X5',Y)) && Valid(ToSSARight(XL1i,XL2i,XL3i,XL4i,X1,X2,X3,X4,S',XL4f,XL5f,Y)) &&
+		EquivalentStatments(ToSSALeft(S,XL3i,XL4f,XL5f,X3,X4,X5,Y),ToSSARight(XL1i,XL2i,XL3i,XL4i,X1,X2,X3,X4,S',XL4f,XL5f,Y));// by {
+}/
+/*
+/*	
+not sure about the parameters to D3, should figure it out and fix; and then
+should show that the preconditions above indeed guarantee that the preconditions of D3 (below, after the appropriate parameter substitutions) all hold;
+and finally show that the postcondition of D3 (again, with the appropriate substitution) guarantee that our postconditions hold.
+
+D.3:
+	Live(XL2f+Y,SeqComp(IF(B,S1,S2),Assignment(XL2f,seqVarToSeqExpr(X2))))
+==
+	Live(XL2f+Y,SeqComp(Assignment(XL1i,seqVarToSeqExpr(X1)),IF(B',S1',S2')))
+
+
+*/
+		var XL1i',XL2f',X1',X2' := setOf(XL1i+XL2i+XL3i+XL4i),X1+X2+X3+X4,
+		assert TransformationD3Left(B,S1,S2,X2,XL2f,Y),TransformationD3Right(B',S1',S2',X1,XL1i,XL2f,Y) && 
+			EquivalentStatments(TransformationD3Left(B,S1,S2,X2,XL2f,Y),TransformationD3Right(B',S1',S2',X1,XL1i,XL2f,Y)) by {
+		TransformationD3(B,B',S1,S2,S1',S2',X1,X2,XL1i,XL2i,XL2f,Y);
+
+/*
+requires Valid(Live(XL2f+Y,SeqComp(S2,Assignment(XL2f,seqVarToSeqExpr(X2)))))
+	requires Valid(Live(XL2f+Y,SeqComp(Assignment(XL1i,seqVarToSeqExpr(X1)),S2')))
+	requires EquivalentStatments(Live(XL2f+Y,SeqComp(S2,Assignment(XL2f,seqVarToSeqExpr(X2)))),
+		Live(XL2f+Y,SeqComp(Assignment(XL1i,seqVarToSeqExpr(X1)),S2'))) // P5
+	requires Valid(Live(XL2f+Y,SeqComp(S1,Assignment(XL2f,seqVarToSeqExpr(X2)))))
+	requires Valid(Live(XL2f+Y,SeqComp(Assignment(XL1i,seqVarToSeqExpr(X1)),S1')))
+	requires EquivalentStatments(Live(XL2f+Y,SeqComp(S1,Assignment(XL2f,seqVarToSeqExpr(X2)))),
+		Live(XL2f+Y,SeqComp(Assignment(XL1i,seqVarToSeqExpr(X1)),S1'))) // P4
+	requires setOf(XL1i) !! B.1 // P3
+	requires setOf(XL1i) !! setOf(X1) // P2
+	requires |X1| == |XL1i|
+	requires EquivalentBooleanExpressions(B',BSubstitute(B,X1,XL1i)) // P1
+
+	requires Valid(TransformationD3Left(B,S1,S2,X2,XL2f,Y))
+	requires Valid(TransformationD3Right(B',S1',S2',X1,XL1i,XL2f,Y))
+	ensures EquivalentStatments(TransformationD3Left(B,S1,S2,X2,XL2f,Y),
+			TransformationD3Right(B',S1',S2',X1,XL1i,XL2f,Y))
+			*/
+	}	
+	assert setOf(X) !! glob(S'); // Q2
+}*/
+*/
+
+function TransformationD3Left(B: BooleanExpression, 
+		S1: Statement, S2: Statement,
+		X2: seq<Variable>,
+		XL2f: seq<Variable>, Y: seq<Variable>): Statement
+{
+	Live(XL2f+Y,SeqComp(IF(B,S1,S2),Assignment(XL2f,seqVarToSeqExpr(X2))))
+}
+
+function TransformationD3Right(B': BooleanExpression, 
+		S1': Statement, S2': Statement,
+		X1: seq<Variable>,
+		XL1i: seq<Variable>, XL2f: seq<Variable>, Y: seq<Variable>): Statement
+{
+	Live(XL2f+Y,SeqComp(Assignment(XL1i,seqVarToSeqExpr(X1)),IF(B',S1',S2')))
+}
+
+lemma TransformationD3(B: BooleanExpression, B': BooleanExpression, 
+		S1: Statement, S2: Statement, S1': Statement, S2': Statement,
+		X1: seq<Variable>, X2: seq<Variable>,
+		XL1i: seq<Variable>, XL2i: seq<Variable>, XL2f: seq<Variable>, Y: seq<Variable>)
+	requires Valid(Live(XL2f+Y,SeqComp(S2,Assignment(XL2f,seqVarToSeqExpr(X2)))))
+	requires Valid(Live(XL2f+Y,SeqComp(Assignment(XL1i,seqVarToSeqExpr(X1)),S2')))
+	requires EquivalentStatments(Live(XL2f+Y,SeqComp(S2,Assignment(XL2f,seqVarToSeqExpr(X2)))),
+		Live(XL2f+Y,SeqComp(Assignment(XL1i,seqVarToSeqExpr(X1)),S2'))) // P5
+	requires Valid(Live(XL2f+Y,SeqComp(S1,Assignment(XL2f,seqVarToSeqExpr(X2)))))
+	requires Valid(Live(XL2f+Y,SeqComp(Assignment(XL1i,seqVarToSeqExpr(X1)),S1')))
+	requires EquivalentStatments(Live(XL2f+Y,SeqComp(S1,Assignment(XL2f,seqVarToSeqExpr(X2)))),
+		Live(XL2f+Y,SeqComp(Assignment(XL1i,seqVarToSeqExpr(X1)),S1'))) // P4
+	requires setOf(XL1i) !! B.1 // P3
+	requires setOf(XL1i) !! setOf(X1) // P2
+	requires |X1| == |XL1i|
+	requires EquivalentBooleanExpressions(B',BSubstitute(B,X1,XL1i)) // P1
+
+	requires Valid(TransformationD3Left(B,S1,S2,X2,XL2f,Y))
+	requires Valid(TransformationD3Right(B',S1',S2',X1,XL1i,XL2f,Y))
+	ensures EquivalentStatments(TransformationD3Left(B,S1,S2,X2,XL2f,Y),
+			TransformationD3Right(B',S1',S2',X1,XL1i,XL2f,Y))
+{
+	var T1 := TransformationD3Left(B,S1,S2,X2,XL2f,Y);
+	var T2 := TransformationD3Right(B',S1',S2',X1,XL1i,XL2f,Y);
+	forall P: Predicate ensures EquivalentPredicates(wp(T1,P),wp(T2,P)) {
+		var P1 := wp(T1,P);
+		var P2 := wp(T2,P);
+		forall s: State | P1.0.requires(s) && P2.0.requires(s) ensures P1.0(s) == P2.0(s) {
+			calc {
+				wp(T2,P).0(s);
+			== // def. of T2 and of TransformationD3Right
+				wp(Live(XL2f+Y,SeqComp(Assignment(XL1i,seqVarToSeqExpr(X1)),IF(B',S1',S2'))),P).0(s);
+			== { assert B'.0(s) == BSubstitute(B,X1,XL1i).0(s); // from P1
+						var IF1,IF1',V := IF(BSubstitute(B,X1,XL1i),S1',S2'),IF(B',S1',S2'),XL2f+Y;
+						assert EquivalentStatments(IF1',IF1);
+						var A1 := Assignment(XL1i,seqVarToSeqExpr(X1));
+						var SC1,SC1' := SeqComp(A1,IF1),SeqComp(A1,IF1');
+						assert EquivalentStatments(SC1',SC1) by { assert EquivalentStatments(IF1',IF1); Leibniz4(A1,IF1,IF1'); }
+						assert EquivalentStatments(Live(V,SC1'),Live(V,SC1));
+						}
+				wp(Live(XL2f+Y,SeqComp(Assignment(XL1i,seqVarToSeqExpr(X1)),IF(BSubstitute(B,X1,XL1i),S1',S2'))),P).0(s);
+			== { assert setOf(XL1i) !! setOf(X1); // P2
+						Law18b(S1',S2',BSubstitute(B,X1,XL1i),[],XL1i,[],seqVarToSeqExpr(X1)); }
+				wp(Live(XL2f+Y,SeqComp(Assignment(XL1i,seqVarToSeqExpr(X1)),IF(BSubstituteVbyE(BSubstitute(B,X1,XL1i),XL1i,seqVarToSeqExpr(X1)),S1',S2'))),P).0(s);
+			== {// remove redundant (reversed) double sub.
+					var B'' := BSubstituteVbyE(BSubstitute(B,X1,XL1i),XL1i,seqVarToSeqExpr(X1));
+					assert EquivalentBooleanExpressions(B,B'') by { assert setOf(XL1i) !! B.1; /* P3 */ ReversedDoubleSubstitutions(B,X1,XL1i); }
+					assert EquivalentStatments(IF(B,S1',S2'),IF(B'',S1',S2'));
+					var A1,IF1,IF1',V := Assignment(XL1i,seqVarToSeqExpr(X1)),IF(B,S1',S2'),IF(B'',S1',S2'),XL2f+Y;
+					var SC1,SC2 := SeqComp(A1,IF1'),SeqComp(A1,IF1);
+					assert EquivalentStatments(SC1,SC2) by { assert EquivalentStatments(IF1',IF1); Leibniz4(A1,IF1',IF1); }
+					assert EquivalentStatments(Live(V,SC1),Live(V,SC2));
+					}
+				wp(Live(XL2f+Y,SeqComp(Assignment(XL1i,seqVarToSeqExpr(X1)),IF(B,S1',S2'))),P).0(s);
+			== { assert setOf(XL1i) !! B.1; // P3
+						Law3(Assignment(XL1i,seqVarToSeqExpr(X1)),S1',S2',B); } // distribute statement over IF
+				wp(Live(XL2f+Y,IF(B,SeqComp(Assignment(XL1i,seqVarToSeqExpr(X1)),S1'),SeqComp(Assignment(XL1i,seqVarToSeqExpr(X1)),S2'))),P).0(s);
+			== { Law21(B,SeqComp(Assignment(XL1i,seqVarToSeqExpr(X1)),S1'),SeqComp(Assignment(XL1i,seqVarToSeqExpr(X1)),S2'),XL2f+Y); } // propagate liveness info.
+				wp(Live(XL2f+Y,IF(B,Live(XL2f+Y,SeqComp(Assignment(XL1i,seqVarToSeqExpr(X1)),S1')),
+					Live(XL2f+Y,SeqComp(Assignment(XL1i,seqVarToSeqExpr(X1)),S2')))),P).0(s);
+			== { var V := XL2f+Y;
+						var T1 := Live(V,SeqComp(S1,Assignment(XL2f,seqVarToSeqExpr(X2))));
+						var T1' := Live(V,SeqComp(Assignment(XL1i,seqVarToSeqExpr(X1)),S1'));
+						assert EquivalentStatments(T1,T1'); // P4
+						var T2 := Live(V,SeqComp(S2,Assignment(XL2f,seqVarToSeqExpr(X2))));
+						var T2' := Live(V,SeqComp(Assignment(XL1i,seqVarToSeqExpr(X1)),S2'));
+						assert EquivalentStatments(T2,T2'); // P5
+						var IF1,IF1' := IF(B,T1,T2),IF(B,T1',T2');
+						assert EquivalentStatments(IF1',IF1);
+						assert EquivalentStatments(Live(V,IF1'),Live(V,IF1));
+					}
+				wp(Live(XL2f+Y,IF(B,Live(XL2f+Y,SeqComp(S1,Assignment(XL2f,seqVarToSeqExpr(X2)))),
+					Live(XL2f+Y,SeqComp(S2,Assignment(XL2f,seqVarToSeqExpr(X2)))))),P).0(s);
+			== { Law21(B,SeqComp(S1,Assignment(XL2f,seqVarToSeqExpr(X2))),SeqComp(S2,Assignment(XL2f,seqVarToSeqExpr(X2))),XL2f+Y); } // remove liveness info.
+				wp(Live(XL2f+Y,IF(B,SeqComp(S1,Assignment(XL2f,seqVarToSeqExpr(X2))),SeqComp(S2,Assignment(XL2f,seqVarToSeqExpr(X2))))),P).0(s);
+			== { Law4(S1,S2,Assignment(XL2f,seqVarToSeqExpr(X2)),B); } // dist. IF over ";"
+				wp(Live(XL2f+Y,SeqComp(IF(B,S1,S2),Assignment(XL2f,seqVarToSeqExpr(X2)))),P).0(s);
+			== // def. of T1 and of TransformationD3Left
+				wp(T1,P).0(s);
+			}
+		}
+	}
+}
+
+//method TransformationD5(S: Statement, X: seq<Variable>, X: seq<Variable>) returns (S': Statement)
+
+function IfToSSACorrectnessLeft(B: BooleanExpression, S1: Statement, S2: Statement,
+		X3: seq<Variable>, X4: seq<Variable>, X5: seq<Variable>, // live-on-exit variables (the X2 of D.3)
+		XL3i: seq<Variable>, XL4f: seq<Variable>, XL5f: seq<Variable>, // live-on-exit instances (the XL2f of D.3)
+		Y: seq<Variable>): Statement
+{
+//	Live(XL3i+XL4f+XL5f+Y,SeqComp(IF(B,S1,S2),Assignment(XL3i+XL4f+XL5f,seqVarToSeqExpr(X3+X4+X5))))
+	TransformationD3Left(B,S1,S2,X3+X4+X5,XL3i+XL4f+XL5f,Y)
+//	Live(XL2f          +Y,SeqComp(IF(B,S1,S2),Assignment(XL2f          ,seqVarToSeqExpr(X2      ))))
+}
+
+function IfToSSACorrectnessRight(B': BooleanExpression, S1': Statement, S2': Statement,
+		X1: seq<Variable>, X2: seq<Variable>, X3: seq<Variable>, X4: seq<Variable>, // live-on-entry variables (the X1 of D.3)
+		XL1i: seq<Variable>, XL2i: seq<Variable>, XL3i: seq<Variable>, XL4i: seq<Variable>, // live-on-entry instances (the XL1i of D.3)
+		XL4f: seq<Variable>, XL5f: seq<Variable>, // along with XL1i: live-on-exit instances (the XL2f of D.3)
+		Y: seq<Variable>): Statement
+{
+//	Live(XL3i+XL4f+XL5f+Y,SeqComp(Assignment(XL1i+XL2i+XL3i+XL4i,seqVarToSeqExpr(X1+X2+X3+X4)),IF(B',S1',S2')))
+	TransformationD3Right(B',S1',S2',X1+X2+X3+X4,XL1i+XL2i+XL3i+XL4i,XL3i+XL4f+XL5f,Y)
+//	Live(XL2f          +Y,SeqComp(Assignment(XL1i               ,seqVarToSeqExpr(X1         )),IF(B',S1',S2')))
+}
+
+lemma IfToSSACorrectness(B: BooleanExpression, S1: Statement, S2: Statement, B': BooleanExpression, S1': Statement, S2': Statement,
+		X1: seq<Variable>, X2: seq<Variable>, X3: seq<Variable>, X4: seq<Variable>, // live-on-entry variables (the X1 of D.3)
+		X5: seq<Variable>, // along with X3,X4: live-on-exit variables (the X2 of D.3)
+		XL1i: seq<Variable>, XL2i: seq<Variable>, XL3i: seq<Variable>, XL4i: seq<Variable>, // live-on-entry instances (the XL1i of D.3)
+		XL4f: seq<Variable>, XL5f: seq<Variable>, // along with XL1i: live-on-exit instances (the XL2f of D.3)
+		Y: seq<Variable>)
+	requires Valid(IfToSSACorrectnessLeft(B,S1,S2,X3,X4,X5,XL3i,XL4f,XL5f,Y))
+	requires Valid(IfToSSACorrectnessRight(B',S1',S2',X1,X2,X3,X4,XL1i,XL2i,XL3i,XL4i,XL4f,XL5f,Y))
+	ensures EquivalentStatments(IfToSSACorrectnessLeft(B,S1,S2,X3,X4,X5,XL3i,XL4f,XL5f,Y),
+			IfToSSACorrectnessRight(B',S1',S2',X1,X2,X3,X4,XL1i,XL2i,XL3i,XL4i,XL4f,XL5f,Y))
